wip

proof/correctness/Correctness_WOTS.ec
@@ -66,6 +66,182 @@ qed.
 
 (** -------------------------------------------------------------------------------------------- **)
 
+module ThashF = {
+  proc thash_f (t : nbytes, seed : seed, address : adrs) : (nbytes * adrs) = {
+    var key : nbytes;
+    var bitmask : nbytes;
+    var addr_bytes : nbytes;
+    
+    addr_bytes <- addr_to_bytes address;
+    key <@ Hash.prf(addr_bytes, seed);
+    address <- set_key_and_mask address 1;
+    addr_bytes <- addr_to_bytes address;
+    bitmask <@ Hash.prf(addr_bytes, seed);
+    t <@ Hash._F(key, nbytexor t bitmask);
+    return (t, address);
+  }
+}.
+
+lemma thash_f_equiv (_out_ _seed_ : W8.t Array32.t) (a : W32.t Array8.t) :
+    n = XMSS_N /\
+    prf_padding_val = XMSS_HASH_PADDING_PRF /\
+    padding_len = XMSS_PADDING_LEN /\ 
+    F_padding_val = XMSS_HASH_PADDING_F =>
+    equiv [
+      M(Syscall).__thash_f ~ ThashF.thash_f :
+      arg{1}.`1 = _out_ /\
+      arg{1}.`2 = _seed_ /\
+      arg{1}.`3 = a /\
+      
+      arg{2}.`1 = NBytes.insubd (to_list _out_) /\
+      arg{2}.`2 = NBytes.insubd (to_list _seed_) /\
+      arg{2}.`3 = a
+      ==>
+      to_list res{1}.`1 = val res{2}.`1 /\
+      res{1}.`2 = res{2}.`2 /\
+      res{1}.`2.[7] = W32.one /\
+      sub res{1}.`2 0 7 = sub a 0 7
+    ].
+proof. 
+rewrite /XMSS_N. 
+move => [#] n_val ???.
+proc => /=.
+seq 4 0 : #pre; first by auto.
+
+seq 1 1 : (#pre /\ to_list addr_as_bytes{1} = val addr_bytes{2}).
+  + by ecall {1} (addr_to_bytes_correctness addr{1}); auto.
+
+inline {2} Hash._F. 
+
+swap {2} 7 -6.
+
+seq 2 1 : (#pre /\ to_list padding{1} = padding{2}).
+  + auto.
+    ecall {1} (ull_to_bytes_32_correct W64.zero).
+    auto => /> &1 &2 ??->. 
+    congr => /#.
+
+seq 1 0 : (#pre /\ sub buf{1} 0 n = padding{2}).
+  + auto => /> &1 &2 ?.
+    apply (eq_from_nth witness); first by rewrite size_to_list n_val size_sub.
+    rewrite n_val size_sub // => j?.
+    by rewrite get_to_list nth_sub // initiE 1:/# /= ifT.
+
+seq 1 1 : (#pre /\ to_list aux{1} = val key{2}).
+  + inline {1} M(Syscall).__prf_ M(Syscall)._prf; wp; sp.
+    exists * in_00{1}, key0{1}; elim * => _P1 _P2.
+    call {1} (prf_correctness _P1 _P2) => [/# |]. 
+    skip => /> &1 &2 H0 H1.
+    split; [smt(@NBytes) | smt()].
+
+seq 1 0 : (#pre /\ sub buf{1} n n = val key{2}).
+  + auto => /> &1 &2 H0 H1 H2. 
+    split.
+      - apply (eq_from_nth witness); first by rewrite n_val size_to_list size_sub.
+        rewrite n_val size_sub // => j?.
+        by rewrite -H1 nth_sub //= initiE 1:/# /= ifF 1:/# nth_sub // n_val .
+      - apply (eq_from_nth witness); first by rewrite valP n_val size_sub.
+        rewrite n_val size_sub // => j?.
+        by rewrite nth_sub // initiE 1:/# /= ifT 1:/# -get_to_list H2. 
+
+seq 1 1 : (
+  #{/~addr{1} = a}{/~address{2} = a}pre /\ 
+  addr{1} = address{2} /\ 
+  addr{1}.[7] = W32.one /\
+  sub addr{1} 0 7 = sub a 0 7
+).
+  + inline {1}; auto => /> &1 &2 H0 H1 H2 H3*.
+    apply (eq_from_nth witness); first by rewrite !size_sub.
+    rewrite size_sub // => j?.
+    by rewrite !nth_sub //= get_setE //= ifF 1:/#.
+
+seq 1 1 : (#pre /\ to_list addr_as_bytes{1} = val addr_bytes{2}).
+  + by ecall {1} (addr_to_bytes_correctness addr{1}); auto. 
+
+seq 1 1 : (#pre /\ to_list bitmask{1} = val bitmask{2}).
+  + inline {1} M(Syscall).__prf_ M(Syscall)._prf; wp; sp.
+    exists * in_00{1}, key0{1}; elim * => _P1 _P2.
+    call {1} (prf_correctness _P1 _P2) => [/# |]. 
+    skip => /> &1 &2 H0 H1 H2 H3 H4 *. 
+    split; [smt(@NBytes) | smt()]. 
+
+seq 2 3 : (
+  addr{1} = address{2} /\
+  addr{1}.[7] = W32.one /\
+  sub addr{1} 0 7 = sub a 0 7 /\
+  to_list buf{1} = buf{2}
+); last first.
+  + auto.
+    inline {1} M(Syscall).__core_hash__96 M(Syscall)._core_hash_96.
+    by wp; sp; ecall {1} (hash_96 in_00{1}); auto => />. 
+
+wp; sp.
+ 
+while {1} 
+(
+  addr{1} = address{2} /\ 
+  addr{1}.[7] = W32.one /\
+  sub addr{1} 0 7 = sub a 0 7 /\
+  0 <= to_uint i{1} <= 32 /\
+  to_list bitmask{1} = val bitmask{2} /\
+  to_list out{1} = val t{2} /\
+  sub buf{1} 0 n = padding{2} /\
+  sub buf{1} n n = val key{2} /\
+  sub buf{1} (n + n) (to_uint i{1}) = sub_list (val (nbytexor t{2} bitmask{2})) 0 (to_uint i{1}) 
+)
+(32 - to_uint i{1}); last first.
+  + auto => /> &1 &2 H0 H1 H2 H3 H4 H5 *.
+    do split. 
+      - by rewrite  insubdK // /P size_to_list n_val.
+      - apply (eq_from_nth witness); first by rewrite size_sub_list // size_sub.
+        rewrite size_sub // => j? /#.
+      - move => bufL iL.
+        split => [* |]; first by rewrite ultE /#.
+        rewrite ultE of_uintK n_val /= => ??? H6 H7 H8 H9 *.
+        apply (eq_from_nth witness); first by by rewrite !size_cat !size_to_list !valP n_val.
+        rewrite size_to_list => j?.
+        case (0 <= j < 32) => ?.
+           + rewrite get_to_list.
+             have ->: bufL.[j] = nth witness (sub bufL 0 32) j by rewrite nth_sub.
+             by rewrite H6 !nth_cat !size_cat !size_to_list !valP n_val /= ifT 1:/# ifT 1:/# H7 get_to_list.
+        case (32 <= j < 64) => ?.
+           + rewrite get_to_list.
+             have ->: bufL.[j] = nth witness (sub bufL 32 32) (j - 32) by rewrite nth_sub /#.
+             by rewrite H8 !nth_cat !size_cat !size_to_list !valP n_val /= ifT 1:/# ifF 1:/#.
+        rewrite get_to_list.
+        have ->: bufL.[j] = nth witness (sub bufL 64 (to_uint iL)) (j - 64) by rewrite nth_sub /#.
+        rewrite H9 !nth_cat !size_cat !size_to_list !valP n_val /= ifF 1:/#.
+        by rewrite /sub_list nth_mkseq 1:/#.
+
+auto => /> &hr H0 H1 H2 H3 H4 H5 H6 H7 H8 *.
+do split; 1,2,6: by smt(@W64 pow2_64).
+  - apply (eq_from_nth witness); first by rewrite !size_sub /#.
+    rewrite size_sub 1:/# => j?.        
+    rewrite !nth_sub //= get_setE; first by smt(@W64 pow2_64).
+    rewrite ifF // to_uintD of_uintK /=/#.
+  - apply (eq_from_nth witness); first by rewrite valP size_sub /#.
+    rewrite size_sub 1:/# => j?.        
+    rewrite !nth_sub //= get_setE; first by smt(@W64 pow2_64).
+    rewrite ifF; first by rewrite to_uintD of_uintK /=/#.
+    rewrite -H6 n_val /= nth_sub /#.
+  - apply (eq_from_nth witness); first by rewrite size_sub to_uintD_small 1..3:/# size_sub_list /#.
+    rewrite size_sub to_uintD_small 1..3:/# => j?.
+    rewrite nth_sub // /sub_list nth_mkseq // /= get_setE; first by smt(@W64 pow2_64).
+    case (to_uint i{hr} = j) => H; [rewrite ifT; first by smt(@W64 pow2_64) | rewrite ifF; first by smt(@W64 pow2_64)]; last first.
+        + rewrite n_val /=.
+          have ->: buf{hr}.[64 + j] = nth witness (sub buf{hr} (n + n) (to_uint i{hr})) j by rewrite nth_sub 2:/#; smt(@W64 pow2_64).
+          rewrite H7 /sub_list nth_mkseq 2:/#; smt(@W64 pow2_64).
+        + rewrite /nbytexor insubdK /bytexor; first by rewrite /P size_map size_zip !valP.
+          rewrite (nth_map witness) /=. 
+             - rewrite size_zip !valP n_val (: min 32 32 = 32) 1:/#; smt(@W64 pow2_64).
+               rewrite zip_fst; first by rewrite !valP n_val /=; smt(@W64 pow2_64).
+               rewrite zip_snd; first by rewrite !valP n_val /=; smt(@W64 pow2_64).
+               rewrite -H4 -!get_to_list H; congr. (* this gets rid of the rhs *)
+               congr.               
+qed.
+
+(** -------------------------------------------------------------------------------------------- **)
+
 lemma base_w_results_64 ( _in_ : W8.t Array32.t) :
     floor (log2 w%r) = XMSS_WOTS_LOG_W /\ 
     w = XMSS_WOTS_W => 
@@ -311,14 +487,14 @@ lemma gen_chain_inplace_correct (_buf_ : W8.t Array32.t, _start_ _steps_ : W32.t
       val res{2} = to_list res{1}.`1 /\
       sub res{1}.`2 0 6 = sub _addr_ 0 6 /\
       res{1}.`2.[7] = W32.one /\
-      res{1}.`2.[6] = _steps_ - W32.one
+      res{1}.`2.[6] = _start_ + _steps_ - W32.one
     ].
 proof. 
 rewrite /XMSS_N /XMSS_WOTS_W.
 move => [#] n_val w_val????. 
 proc => //=.
 swap {1} 1 2.
-
+ 
 seq 2 1 : ( 
   0 <= to_uint start{1} <= w - 1/\
   0 <= to_uint steps{1} <= w - 1 /\
@@ -338,17 +514,111 @@ seq 2 1 : (
       rewrite w_val.
       do 3! (split => [/# |]); do split; by rewrite NBytes.insubdK /P // size_to_list n_val.
 
-(* We unroll the first iteration on both sides so that the invariant is easier to write *)
-(* stupid but works *)
-
 sp 1 1.
+
+unroll {1} 1; unroll {2} 1.
+rcondt {2} 1; first by auto => /> /#. 
+rcondt {1} 1; first by auto => /> &hr *; rewrite ultE to_uintD /#.
+
+seq 2 2 : (
+    #{/~addr{1} = _addr_}pre /\
+    addr{1}.[6] = i{1}
+); first by inline {1}; auto.
+
+outline {2} [1-6] { (t, address) <@ ThashF.thash_f (t, _seed, address); }.
+
+
+seq 1 1 : (#pre /\ to_list out{1} = val t{2} /\ addr{1}.[7] = W32.one); last by admit.
+    + inline M(Syscall).__thash_f_ M(Syscall)._thash_f; wp; sp.
+      exists * out1{1}, pub_seed1{1}, addr{1}.
+      elim * => P0 P1 P2.
+      call (thash_f_equiv P0 P1 P2) => [/# |].
+      auto => /> &1 &2 *.
+      do split => //=; 1,2: by smt(@NBytes).
+      move => H0 H1 H2 H3 H4 H5 H6 *.
+      do split; 1..3: by smt().
+smt().smt().
+smt().
+smt().
+
+
+
+   
+
+
+
+      
+inline {1} 1.
+
+while ( 
+  ((0 < chain_count{2}) => addr{1}.[6] = i{1}) /\
+  sub addr{1} 0 6 = sub _addr_ 0 6 /\
+  val t{2} = to_list out{1} /\
+  0 <= to_uint start{1} <= w - 1/\
+  0 <= to_uint steps{1} <= w - 1 /\
+  0 <= to_uint (start{1} + steps{1}) <= w - 1 /\
+  to_uint start{1} < to_uint start{1} + to_uint steps{1} /\
+  address{2} = addr{1} /\ 
+  to_uint start{1} <= to_uint i{1} <= to_uint start{1} + to_uint steps{1} /\
+  t{1} = start{1} + steps{1} /\
+  to_uint i{1} = i{2} + chain_count{2} /\
+  0 <= chain_count{2} <= s{2} 
+); last first.
+    + auto => /> &1 &2 *.
+      rewrite !ultE to_uintD. 
+      do split; 1..3: by smt().
+      move => addrL iL outL chaincountR t.
+      rewrite ultE -!lezNgt => ????? *.
+      split => [/# |].
+      admit.
+ 
+seq 2 2 : #pre; last by admit.
+    + inline {1}; auto => &1 &2. 
+      rewrite ultE.
+      move => [#] H0 H1 H2 H3 H4 H5 H6 H7 H8 H9 H10 H11 H12 H13 H14 H15 H16 H17 H18 H19 addrL *.
+      do split => //. (* => // reduces the number of subgoals from 19 to 3 *)
+       - move => ?.
+         rewrite /addrL !get_setE //=.
+       - apply (eq_from_nth witness); first by rewrite !size_sub. 
+         rewrite size_sub // => j?.
+         by rewrite -H2 !nth_sub //= /addrL !get_setE //= ifF 1:/# ifF 1:/#.
+       - rewrite tP => j?.
+         rewrite /set_key_and_mask /set_hash_addr /addrL !get_setE //. 
+         case (j = 7) => //?.
+         case (j = 6) => ?; first by rewrite -H15 to_uintK.
+         smt(sub_k).
+       
+
+
+
+
+
+
 
 unroll {1} 1; rcondt {1} 1.
     + auto => /> &hr *. 
       by rewrite ultE to_uintD_small 1:/#. 
 
+
+
+
 unroll {2} 1; rcondt {2} 1; first by auto => /> /#. 
+
+seq 2 2 : (#{/~addr{1} = _addr_}pre); first by inline {1}; auto.
+      
+seq 1 6 : (
+  #pre /\
+  to_list out{1} = val t{2} /\
+  sub addr{1} 0 6 = sub address{2} 0 6
+).
+    + inline M(Syscall).__thash_f_ M(Syscall)._thash_f.
+
 admit.
+
+while (
+  (to_uint start{2} < to_uint i{1}
+); first by admit.
+
 qed.
 
 
